Introduce InvDeriv to examples.logic

nola/examples/logic.v
@@ -1,8 +1,8 @@
 (** * Showcase logic *)
 
-From nola.iris Require Import ciprop inv.
+From nola.iris Require Import ciprop inv_deriv.
 From nola.heap_lang Require Import notation proofmode.
-Import WpwNotation iPropAppNotation.
+Import WpwNotation iPropAppNotation PintpNotation.
 
 Implicit Type (N : namespace) (l : loc).
 
@@ -45,26 +45,51 @@ Section ciProp.
   Proof. move=> ????. apply cip_custom_ne; solve_proper. Qed.
 End ciProp.
 
+(** ** [judg]: Judgment *)
+Definition judg Σ : ofe := prodO (leibnizO namespace) (ciProp Σ).
+Definition inv_jacsr {Σ} N P : judg Σ := (N, P).
+#[export] Instance inv_jacsr_ne {Σ N} : NonExpansive (@inv_jacsr Σ N).
+Proof. done. Qed.
+
+#[export] Instance judg_inv_pre_deriv {Σ} :
+  InvPreDeriv (ciProp Σ) (judg Σ) := INV_PRE_DERIV inv_jacsr.
+
 Section iris.
   Context `{!inv'GS ciPropOF Σ}.
+  Implicit Type δ : judg Σ → iProp Σ.
 
   (** ** [bintp]: Base interpretation *)
-  Definition bintp s : (idom s -d> iProp Σ) → (cdom s -d> ciProp Σ) →
+  Definition bintp δ s : (idom s -d> iProp Σ) → (cdom s -d> ciProp Σ) →
     dataOF s $oi Σ → iProp Σ :=
     match s with
-    | cips_inv N => λ _ Pxs _, inv_tok N (Pxs ())
+    | cips_inv N => λ _ Pxs _, inv' δ N (Pxs ())
     end.
 
   (** [bintp] is non-expansive *)
-  #[export] Instance bintp_ne {s} : NonExpansive3 (bintp s).
-  Proof. case s=>/= ??????? eqv ???. f_equiv. apply eqv. Qed.
+  #[export] Instance bintp_ne `{!NonExpansive δ} {s} :
+    NonExpansive3 (bintp δ s).
+  Proof. case s; solve_proper. Qed.
 
-  (** ** [intp]: Interpretation of [ciProp] *)
-  Definition intp : ciProp Σ → iProp Σ := cip_intp bintp.
+  (** ** Parameterized interpretation of [ciProp] *)
+  #[export] Instance ciProp_dintp : Dintp (judg Σ) (ciProp Σ) (iProp Σ) :=
+    DINTP (λ δ, cip_intp (bintp δ)).
 
-  (** [intp] is non-expansive *)
-  Fact intp_ne : NonExpansive intp.
+  (** [ciProp_intp] is non-expansive *)
+  Fact ciProp_intp_ne `{!NonExpansive δ} : NonExpansive ⟦⟧(δ)@{ciProp Σ}.
   Proof. exact _. Qed.
+
+  Context `{!invGS_gen hlc Σ}.
+
+  (** ** [jintp]: Judgment interpretation *)
+  Definition jintp δ (J : judg Σ) := match J with
+    | (N, Px) => inv_acsr ⟦⟧(δ) N ⟦ Px ⟧(δ)
+    end.
+  Local Instance jintp_ne `{!NonExpansive δ} : NonExpansive (jintp δ).
+  Proof. move=> ?[??][??][/=??]. solve_proper. Qed.
+  Canonical judgJ : judgi (iProp Σ) := Judgi _ jintp.
+
+  #[export] Instance judg_inv_deriv : InvDeriv ciPropOF Σ judgJ.
+  Proof. done. Qed.
 End iris.
 
 (** ** Target function: Linked list mutation *)
@@ -90,10 +115,10 @@ Section iris.
   (** ** Termination of [iter] *)
   Lemma twp_iter {N Φ c l} {f : val} {n : nat} :
     (∀ l0 : loc,
-      [[{ inv_tok N (Φ l0) }]][inv_wsat intp]
+      [[{ inv' der N (Φ l0) }]][inv_wsatd der]
         f #l0 @ ↑N
       [[{ RET #(); True }]]) -∗
-    [[{ c ↦ #n ∗ intp (ilist N Φ l) }]][inv_wsat intp]
+    [[{ c ↦ #n ∗ ⟦ ilist N Φ l ⟧(der) }]][inv_wsatd der]
       iter f #c #l @ ↑N
     [[{ RET #(); c ↦ #0 }]].
   Proof.
@@ -103,8 +128,8 @@ Section iris.
     wp_rec. wp_pures. wp_load. wp_pures. wp_apply "Hf"; [done|]. iIntros "_".
     wp_pures. wp_load. wp_op. have -> : (S m - 1)%Z = m by lia. wp_store.
     wp_op. wp_bind (! _)%E.
-    iMod (inv_tok_acc (PROP:=ciPropOF) (intp:=intp) with "itl") as
-      "/=[(%l' & >↦l' & #itlhd & #itltl) cl]/="; [done|].
+    iMod (inv'_acc with "itl") as "/=[(%l' & >↦l' & #itlhd & #itltl) cl]/=";
+      [done|].
     wp_load. iModIntro. iMod ("cl" with "[↦l']") as "_".
     { iExists _. iFrame "↦l'". by iSplit. }
     iModIntro. by iApply ("IH" with "c↦ HΨ").
